Fixed a bug in feval that would step malformed expressions. Lots of progress on the proof of correctness for the f_apply case.

FEV_Definitions.v
@@ -71,7 +71,12 @@ Fixpoint feval (e:fexp) (fct:fctable) : option fexp :=
   match e with
   | f_apply e1 e2 =>
     match feval e2 fct with
-    | Some e2' => Some (f_apply e1 e2') (* RC-INVK-ARG, RC-NEW-ARG *)
+    | Some e2' =>
+      match e1 with
+      | f_var v => None      (* Can't step arguments unless well-formed *)
+      | f_field e fn => None
+      | e1 => Some (f_apply e1 e2') (* RC-INVK-ARG, RC-NEW-ARG *)
+      end
     | None =>
       match feval e1 fct with
       | Some e1' => Some (f_apply e1' e2) (* RC-INVK-RECV *)
